Modification of GRA defs

iris_system/lib/allocs.v
@@ -6,14 +6,15 @@ Definition allocsR (A : cmra) : cmra :=
 Definition allocsUR (A : cmra) : ucmra :=
   positive -d> optionUR (csumR (exclR unitO) A).
 
-Definition allocs_auth (A : cmra) (u : positive) : allocsR A :=
-  λ γ, if decide (γ < u)%positive then None else Some (Cinl (Excl tt)).
+Definition allocs_auth (A : cmra) (P : positive → Prop) `{∀ p, Decision (P p)} : allocsR A :=
+  λ γ, if decide (P γ) then Some (Cinl (Excl tt)) else None.
 Definition allocs_frag {A : cmra} γ a : allocsR A :=
   discrete_fun_singleton γ (Some (Cinr a)).
 Global Instance: Params (@allocs_frag) 4 := {}.
+Global Arguments allocs_auth A P {_}.
 
 Section allocs.
-  Context {A : cmra}.
+  Context `{CmraDiscrete A}.
   Implicit Types a b : A.
   Implicit Types γ : positive.
 
@@ -30,16 +31,27 @@ Section allocs.
   Proof. by rewrite discrete_fun_singleton_valid Some_valid Cinr_valid. Qed.
 
   (** Frame-preserving updates *)
-  Lemma allocs_alloc u a (WF : ✓ a) : allocs_auth A u ~~> allocs_auth A (u + 1) ⋅ allocs_frag u a.
+  (* TODO : This can be further generalized to yielding list of resources. *)
+  Lemma allocs_alloc a `{∀ p, Decision (P p)} `{∀ p, Decision (Q p)}
+      (WF : ✓ a) (EX : ∃ γ, P γ ∧ ~ Q γ) (INCL : ∀ γ, Q γ → P γ) :
+    ∃ γ, allocs_auth A P ~~> allocs_auth A Q ⋅ allocs_frag γ a.
   Proof.
+    destruct EX as [γ [HP HNQ]]; exists γ.
     apply discrete_fun_update; intros p; rewrite discrete_fun_lookup_op ?/allocs_auth /allocs_frag.
-    destruct (decide (p < u))%positive.
-    { rewrite discrete_fun_lookup_singleton_ne; des_ifs; lia. }
-    { des_ifs; rewrite ?left_id.
-      { assert (u = p) by lia; subst; rewrite discrete_fun_lookup_singleton.
-        by apply option_update, cmra_update_exclusive.
+    des_ifs.
+    { rewrite discrete_fun_lookup_singleton_ne; ss. ii; clarify; ss. }
+    { rewrite left_id.
+      destruct (decide (γ = p)); clarify;
+        [rewrite discrete_fun_lookup_singleton | rewrite discrete_fun_lookup_singleton_ne]; ss.
+      { apply option_update, cmra_update_exclusive; ss. }
+      { rewrite cmra_discrete_total_update.
+        intros [z|]; ss; rewrite left_id -Some_op; intros CONT%exclusive_l; ss.
+        apply Cinl_exclusive; ss.
       }
-      { rewrite discrete_fun_lookup_singleton_ne; try lia; ss. }
+    }
+    { naive_solver. }
+    { destruct (decide (γ = p)); clarify.
+      rewrite discrete_fun_lookup_singleton_ne; ss.
     }
   Qed.
 End allocs.
