modules/index.v
@@ -1,6 +1,0 @@
-(** * Module index typeclass, for composing modules and their simulation proofs *)
-From stdpp Require Import numbers.
-
-Class mod_index : Type := mod_index_mk {
-  mod_index_elem : positive
-}.
